---
title: 2.1 The Derivative and the Tangent Line Problem
---

## {{ page.title }}

What we did with limits, understanding what it means to approach something even if you can't get there, starts to pay off here. The fundamental problem that opens up the next chapter of mathematics is the tangent line problem. How can you determine the slope of the line that is tangent to a curve? This hurdle was collectively worked on so much that multiple people solved it at nearly the same exact time in different parts of the world. If you're curious about that history, this is a good place to start: [Leibnizâ€“Newton calculus controversy](https://en.wikipedia.org/wiki/Leibniz%E2%80%93Newton_calculus_controversy)

As for the tangent line problem itself, you can approximate the tangent line with a secant line by just having the points really close to each other. We'll call that distance $\Delta x$ and then our two points will be 

$$ (c,f(c)) \quad\text{and}\quad (c+\Delta x, f(c+\Delta x))$$

Now we can use our slope formula to come up with the slope of that secant line.

$$\begin{align*}
m       &= \frac{y_2-y_1}{x_2-x_1} \\[1em]
m_{sec} &= \frac{f(c+\Delta x) - f(c)}{(c+\Delta x) - c}\\[1em]
m_{sec} &= \frac{f(c+\Delta x) - f(c)}{\Delta x}
\end{align*}$$

This leads us to our definition of a tangent line. Since we want those two points to be as close as possible

$$ \lim_{\Delta x \to 0} \frac{f(c+\Delta x) - f(c)}{\Delta x} $$

Let's apply that to something we couldn't normally get the slope of, a quadratic: $f(x)=x^2+1$ at the point $(-1,2)$.

$$\begin{align*}
\lim_{\Delta x \to 0} \frac{f(-1+\Delta x) - f(-1)}{\Delta x} &=
    \lim_{\Delta x \to 0} \frac{(1-2\Delta x+\Delta x^2) + 1 - 2}{\Delta x} \\[1em]
&= \lim_{\Delta x \to 0} \frac{-2\Delta x+\Delta x^2}{\Delta x} \\[1em]
&= \lim_{\Delta x \to 0} -2 + \Delta x \\[1em]
&= -2
\end{align*}$$

In fact, you could do this in general for any point in the function.

$$\begin{align*}
\lim_{\Delta x \to 0} \frac{f(c+\Delta x) - f(c)}{\Delta x} &=
    \lim_{\Delta x \to 0} \frac{(c^2+2c\Delta x+\Delta x^2) + 1 - (c^2+1)}{\Delta x} \\[1em]
&= \lim_{\Delta x \to 0} \frac{2c\Delta x+\Delta x^2}{\Delta x} \\[1em]
&= \lim_{\Delta x \to 0} 2c + \Delta x \\[1em]
&= 2c
\end{align*}$$

### The Derivative of a Function

